Codigo de nuevas aristas para usar set comprehension

Especificaciones/Auxiliar/SetFacts.dfy
@@ -30,6 +30,11 @@ requires A >= B
 ensures A == B 
 { }
 
+lemma setEquialityDefinition2<T>(A: set<T>, B: set<T>)
+requires forall t: T :: t in A <==> t in B
+ensures A == B 
+{ }
+
 lemma equalityBelonging<T>(A: set<T>, B: set<T>)
 requires A == B 
 ensures forall t: T :: t in A <==> t in B 
@@ -45,6 +50,28 @@ requires A == (set t: T | t in B :: t)
 ensures A == B
 { }
 
+
+lemma sameCardinalThroughComprehension<T>(A: set<T>, B: set<set<T>>)
+decreases A
+requires forall b: set<T> | b in B :: (exists a: T, c: T :: a in A && c !in A && b == {a, c}) 
+requires forall a: T | a in A :: exists b: set<T> :: b in B && a in b && (forall b': set<T> | b' in B && a in b' :: b == b')
+ensures |A| == |B|
+{ 
+  if A == {} {}
+  else{
+    var a :| a in A;
+    var b :| b in B && a in b;
+    var A' := A - {a};
+    var B' := B - {b};
+    sameCardinalThroughComprehension(A - {a}, B - {b});
+  }
+}
+
+lemma strictSubsetDefinition<T>(A: set<T>, B: set<T>)
+requires A < B 
+ensures exists b: T :: b in B && b !in A 
+{ }
+
 lemma cardinalityLemma1()
 ensures forall A, B: set<nat> :: (A >= B ==> |A - B| == |A| - |B|)
 { }
@@ -55,14 +82,26 @@ ensures forall A, B: set<nat> :: ( A >= B && |A| == |B| ) ==> A == B
   cardinalityLemma1();
 }
 
-lemma cardinalityLemma3(A: set<nat>, B: set<nat>)
+lemma subsetCardinality<T>(A: set<T>, B: set<T>)
 requires A <= B
 ensures |A| <= |B|
 {
   if A == {} {} 
   else {
+    ghost var x: T :| x in A;
+    subsetCardinality(A - {x}, B - {x}); 
+  } 
+}
+
+lemma strictSubsetCardinality(A: set<nat>, B: set<nat>)
+requires A < B
+requires B != {}
+ensures |A| < |B|
+{
+  if A == {} {} 
+  else {
     ghost var x: nat :| x in A;
-    cardinalityLemma3(A - {x}, B - {x}); 
+    strictSubsetCardinality(A - {x}, B - {x}); 
   } 
 }
 
@@ -88,10 +127,49 @@ lemma cardinalityLemma5(A: set<nat>)
   }
 }
 
+lemma cardinality2implies<T>(A: set<T>, a: T)
+requires |A| > 1
+requires a in A 
+ensures exists b: T :: b in A && b != a 
+{ 
+  if !exists b: T :: b in A && b != a {
+    assert forall x: T | x in A :: x == a;
+    assert A == {a};
+    assert |A| == 1;
+  }
+}
+
 lemma cardinalitySum<T>(A: set<T>, B: set<T>)
 requires A * B == {}
 ensures |A + B| == |A| + |B|
 { }
+
+lemma cardinalityUnion<T>(A: set<T>, B: set<T>, C: set<T>)
+requires A + B == C
+ensures |A| + |B| >= |C|
+ensures |C| >= |A|
+ensures |C| >= |B|
+{ 
+  subsetCardinality(A, C);
+  subsetCardinality(B, C);
+  assert |C| >= |A|;
+  assert |C| >= |B|;
+  assert |C| <= |A| + |B| by {
+    assert |C| > |A| + |B| ==> exists t: T :: t in C && t !in A && t !in B; 
+  }
+}
+
+lemma strictSubsetImpliesLesserCardinal<T>(A: set<T>, B: set<T>)
+requires A > B 
+ensures |A| > |B|
+{ 
+  assert exists a: T :: (a in A && a !in B);
+  var a: T :| (a in A && a !in B);
+  assert a in A - B;
+  assert A - B > {};
+  assert |A - B| >= 1;
+  assert |B - B| == 0;
+}
 
 lemma emptyOverpowersIntersection<T>(A: set<T>, B: set<T>)
 requires A == {}
@@ -243,3 +321,162 @@ decreases k
     //assert !((pickMax(S) + 1) in S);
     {pickMax(S) + 1} + addMultipleGreater({pickMax(S) + 1}, k - 1) 
 }
+
+function numberOfLesser(A: set<nat>, x: nat): (y: nat)
+requires x in A 
+ensures y < |A|
+{
+  var setLesser: set<nat> := (set a: nat | a in A && a < x);
+  assert setLesser <= A;
+  assert pickMax(A) !in setLesser;
+  assert setLesser < A; 
+  strictSubsetCardinality(setLesser, A);
+  |setLesser|
+}
+
+lemma numberOfLesserEquality(A: set<nat>, x: nat, y: nat)
+requires x in A 
+requires y in A 
+requires numberOfLesser(A, x) == numberOfLesser(A, y)
+ensures x == y
+{
+  if x > y {
+    greaterTransitivity(A, x, y);
+    assert numberOfLesser(A, x) > numberOfLesser(A, y);
+  }
+  else if y > x{
+    greaterTransitivity(A, y, x);
+    assert numberOfLesser(A, y) < numberOfLesser(A, x);
+  }
+}
+
+lemma numberOfLesserEqualityForAll(A: set<nat>, x: nat)
+requires x in A 
+ensures forall y: nat | y in A && numberOfLesser(A, x) == numberOfLesser(A, y) :: x == y
+{
+  forall y | y in A && numberOfLesser(A, x) == numberOfLesser(A, y) 
+  ensures x == y {
+    numberOfLesserEquality(A, x, y);
+  }
+}
+
+function pickFromOrder(A: set<nat>, k: nat): (a: nat)
+requires 0 <= k < |A|
+ensures a in A
+ensures numberOfLesser(A, a) == k
+{
+  alwaysOneElementGreaterThanKElements(A, k);
+  assert exists x: nat :: x in A && numberOfLesser(A, x) == k;
+  var x :| x in A && numberOfLesser(A, x) == k;
+  x
+}
+
+lemma corollaryToMin(A: set<nat>, a: nat)
+requires a in A
+requires a == pickMin(A)
+ensures numberOfLesser(A, a) == 0
+{ }
+
+lemma corollaryToMax(A: set<nat>, a: nat)
+requires a in A
+requires a == pickMax(A)
+ensures numberOfLesser(A, a) == |A| - 1
+{
+  var max: nat := pickMax(A);
+  assert forall n: nat | n in A && n != max :: n < max;
+  assert (set a: nat | a in A && a < max) == A - {max};
+}
+
+lemma greaterTransitivity(A: set<nat>, x: nat, y: nat)
+requires x in A && y in A 
+requires x > y
+ensures numberOfLesser(A, x) > numberOfLesser(A, y)
+{ 
+  var setA := (set a: nat | a in A && a < x); 
+  var setB := (set a: nat | a in A && a < y);
+  assert forall a: nat | a in setB :: a < x;
+  assert setA >= setB;
+  assert y in setA && y !in setB;
+  assert setA > setB;
+  strictSubsetImpliesLesserCardinal(setA, setB);
+  assert |setA| > |setB|;
+}
+
+
+lemma alwaysAnElementGreaterThanKElements(A: set<nat>, k: nat)
+decreases |A| - k - 1
+requires 0 <= k < |A|
+ensures exists a: nat :: a in A && numberOfLesser(A, a) == k 
+{
+  assert |A| > k;
+  var max: nat := pickMax(A);
+  corollaryToMax(A, max);
+  assert numberOfLesser(A, max) + 1 == |A|;
+  if k + 1 == |A| {}
+  else{
+    assert numberOfLesser(A, max) > k;
+    assert (exists a: nat :: a in A && numberOfLesser(A, a) == k) <==> (exists a: nat :: a in (A - {max}) && numberOfLesser((A - {max}), a) == k) by {
+      assert numberOfLesser(A, max) != k;
+      if exists a: nat :: a in A && numberOfLesser(A, a) == k {
+        var num: nat :| num in A && numberOfLesser(A, num) == k;
+        assert num != max; 
+        assert num in (A - {max});
+        alwaysAnElementGreaterThanKElements(A - {max}, k);
+        assert (exists a: nat :: a in (A - {max}) && numberOfLesser((A - {max}), a) == k);  
+      }
+      else{
+        forall a: nat | a in A && a != max
+        ensures numberOfLesser(A, a) != k ==> numberOfLesser(A - {max}, a) != k
+        {
+          assert k + 1 != |A|;
+          var setAux := (set num: nat | num in A && num < a);
+          assert |setAux| != k;
+          assert max !in setAux;
+          assert setAux <= A - {max};
+          var setAux' := (set num: nat | num in A - {max} && num < a);
+          assert setAux == setAux';
+          assert |setAux'| != k;
+          assert numberOfLesser(A - {max}, a) != k;
+        }
+      }
+    }
+    alwaysAnElementGreaterThanKElements(A - {max}, k);
+  }
+}
+
+
+lemma alwaysOneElementGreaterThanKElements(A: set<nat>, k: nat)
+decreases k
+requires 0 <= k < |A|
+ensures exists a: nat :: (a in A && numberOfLesser(A, a) == k && (forall b: nat | b in A && numberOfLesser(A, b) == k :: b == a))
+{
+  alwaysAnElementGreaterThanKElements(A, k);
+  var a: nat :| a in A && numberOfLesser(A, a) == k;
+  if exists b: nat :: b in A && numberOfLesser(A, b) == k && b != a {
+    var b: nat :| b in A && numberOfLesser(A, b) == k && b != a; 
+    assert b > a || a > b;
+    if a > b {
+      greaterTransitivity(A, a, b);
+      assert numberOfLesser(A, a) > numberOfLesser(A, b);
+    }
+    else{
+      greaterTransitivity(A, b, a);
+      assert numberOfLesser(A, a) < numberOfLesser(A, b);
+    }
+  }
+}
+/*
+lemma alwaysOneElementGreaterThanKElementsForAll(A: set<nat>)
+ensures forall k: nat | 0 <= k < |A| :: (exists a: nat :: (a in A && numberOfLesser(A, a) == k))// && (forall b: nat | b in A && numberOfLesser(A, b) == k :: a == b)) 
+{
+  forall k: nat | 0 <= k < |A| ensures
+  (exists a: nat :: (a in A && numberOfLesser(A, a) == k)){
+    var a: nat := pickFromOrder(A, k);
+    assert a in A;
+    assert numberOfLesser(A, a) == k;
+  }
+  //duda
+  assume false;
+  assert forall k: nat | 0 <= k < |A|  :: exists a : nat :: a in A && numberOfLesser(A, a) == k;
+}
+*/
